Prettify some of the simply-typed λ-calculus example

examples/lambda/typing/contextlistsScript.sml
@@ -1,151 +1,142 @@
 open HolKernel bossLib boolLib Parse
 
 open nomsetTheory
+open sortingTheory
 
 val _ = new_theory "contextlists"
 
-val _ = type_abbrev("ctxt", ``:(string # 'a) list``)
+Type ctxt = “:(string # 'a) list”
 
 (* permutation over contexts swaps the strings and leaves the types alone *)
-val _ = overload_on
-        ("ctxtswap", ``listpm (pair_pmact string_pmact discrete_pmact)``)
+Overload ctxtswap = “listpm (pair_pmact string_pmact discrete_pmact)”
 
 (* the free variables of a context *)
-val _ = overload_on
-        ("ctxtFV",
-         ``supp (list_pmact (pair_pmact string_pmact discrete_pmact))``)
+Overload ctxtFV =
+         “supp (list_pmact (pair_pmact string_pmact discrete_pmact))”
 
 (* A context is valid if the strings
    are all disjoint.  Here's the primitive recursive defn. *)
-val valid_ctxt_def = Define`
+Definition valid_ctxt_def[simp]:
   (valid_ctxt [] ⇔ T) ∧
   (valid_ctxt ((x,A) :: G) ⇔ x ∉ ctxtFV G ∧ valid_ctxt G)
-`;
-val _ = export_rewrites ["valid_ctxt_def"]
+End
 
 (* here's the alternative characterisation in terms of the standard
    ALL_DISTINCT constant *)
-val valid_ctxt_ALL_DISTINCT = store_thm(
-  "valid_ctxt_ALL_DISTINCT",
-  ``∀G. valid_ctxt G = ALL_DISTINCT (MAP FST G)``,
+Theorem valid_ctxt_ALL_DISTINCT:
+  ∀G. valid_ctxt G = ALL_DISTINCT (MAP FST G)
+Proof
   Induct THEN
   ASM_SIMP_TAC (srw_ss()) [pairTheory.FORALL_PROD, NOT_IN_supp_listpm,
-                           listTheory.MEM_MAP]);
+                           listTheory.MEM_MAP]
+QED
 
-val valid_ctxt_APPEND = store_thm(
-  "valid_ctxt_APPEND",
-  ``valid_ctxt (G1 ++ G2) ==> valid_ctxt G1 ∧ valid_ctxt G2``,
-  Induct_on `G1` THEN
-  ASM_SIMP_TAC (srw_ss()) [pairTheory.FORALL_PROD]);
+Theorem valid_ctxt_APPEND:
+  valid_ctxt (G1 ++ G2) ==> valid_ctxt G1 ∧ valid_ctxt G2
+Proof
+  Induct_on ‘G1’ THEN ASM_SIMP_TAC (srw_ss()) [pairTheory.FORALL_PROD]
+QED
 
 (* context membership "respects" permutation *)
-val MEM_ctxtswap = store_thm(
-  "MEM_ctxtswap",
-  ``!G pi x A. MEM (lswapstr pi x, A) (ctxtswap pi G) = MEM (x,A) G``,
-  SRW_TAC [][MEM_listpm])
-val _ = export_rewrites ["MEM_ctxtswap"]
+Theorem MEM_ctxtswap[simp]:
+  !G pi x A. MEM (lswapstr pi x, A) (ctxtswap pi G) = MEM (x,A) G
+Proof SRW_TAC [][MEM_listpm]
+QED
 
 val ctxtFV_ctxtswap = store_thm(
   "ctxtFV_ctxtswap",
-  ``ctxtFV (ctxtswap pi G) = setpm string_pmact pi (ctxtFV G)``,
+  “ctxtFV (ctxtswap pi G) = setpm string_pmact pi (ctxtFV G)”,
   MATCH_ACCEPT_TAC perm_supp);
 val _ = export_rewrites ["ctxtFV_ctxtswap"]
 
 (* valid_ctxt also respects permutation *)
 val valid_ctxt_swap0 = prove(
-  ``!G. valid_ctxt G ==> !x y. valid_ctxt (ctxtswap pi G)``,
+  “!G. valid_ctxt G ==> !x y. valid_ctxt (ctxtswap pi G)”,
   Induct THEN ASM_SIMP_TAC (srw_ss()) [pairTheory.FORALL_PROD]);
 
 val valid_ctxt_swap = store_thm(
   "valid_ctxt_swap",
-  ``valid_ctxt (ctxtswap pi G) = valid_ctxt G``,
+  “valid_ctxt (ctxtswap pi G) = valid_ctxt G”,
   METIS_TAC [valid_ctxt_swap0, pmact_inverse]);
 val _ = export_rewrites ["valid_ctxt_swap"]
 
 (* contexts have finitely many free variables *)
-val FINITE_ctxtFV = store_thm(
-  "FINITE_ctxtFV",
-  ``FINITE (ctxtFV G)``,
-  Induct_on `G` THEN
-  ASM_SIMP_TAC (srw_ss()) [pairTheory.FORALL_PROD, supp_pairpm]);
-val _ = export_rewrites ["FINITE_ctxtFV"]
+Theorem FINITE_ctxtFV[simp]: FINITE (ctxtFV G)
+Proof
+  Induct_on ‘G’ >> simp[pairTheory.FORALL_PROD, supp_pairpm]
+QED
 
 val ctxtswap_fresh = store_thm(
   "ctxtswap_fresh",
-  ``¬(x ∈ ctxtFV G) /\ ¬(y ∈ ctxtFV G) ==> (ctxtswap [(x,y)] G = G)``,
+  “¬(x ∈ ctxtFV G) /\ ¬(y ∈ ctxtFV G) ==> (ctxtswap [(x,y)] G = G)”,
   MATCH_ACCEPT_TAC supp_fresh)
 
 (* sub-context relation, overloaded to use SUBSET *)
-val subctxt_def = Define`
+Definition subctxt_def:
   subctxt Γ Δ = ∀x A. MEM (x,A) Γ ==> MEM (x,A) Δ
-`;
-val _ = overload_on("SUBSET", ``subctxt``)
+End
+Overload SUBSET = “subctxt”
 
-val subctxt_nil = store_thm(
-  "subctxt_nil",
-  ``[] ⊆ Γ``,
-  SRW_TAC [][subctxt_def]);
-val _ = export_rewrites ["subctxt_nil"]
+Theorem subctxt_nil[simp]: [] ⊆ Γ
+Proof SRW_TAC [][subctxt_def]
+QED
 
-val subctxt_refl = store_thm(
-  "subctxt_refl",
-  ``G : 'a ctxt ⊆ G``,
-  SRW_TAC [][subctxt_def]);
-val _ = export_rewrites ["subctxt_refl"]
+Theorem subctxt_refl[simp]: G : 'a ctxt ⊆ G
+Proof SRW_TAC [][subctxt_def]
+QED
 
 (* cute, but unnecessary *)
 val subctxt_ctxtFV = store_thm(
   "subctxt_ctxtFV",
-  ``C1 ⊆ C2 ==> ctxtFV C1 ⊆ ctxtFV C2``,
+  “C1 ⊆ C2 ==> ctxtFV C1 ⊆ ctxtFV C2”,
   SIMP_TAC (srw_ss()) [pred_setTheory.SUBSET_DEF, subctxt_def,
                        IN_supp_listpm, pairTheory.EXISTS_PROD] THEN
   METIS_TAC []);
 
-open sortingTheory
-val PERM_RULES = LIST_CONJ [Q.SPEC `[]` PERM_REFL,
-                            prove(``∀x l1 l2. PERM l1 l2 ==>
-                                               PERM (x::l1) (x::l2)``,
+val PERM_RULES = LIST_CONJ [Q.SPEC ‘[]’ PERM_REFL,
+                            prove(“∀x l1 l2. PERM l1 l2 ==>
+                                               PERM (x::l1) (x::l2)”,
                                   SRW_TAC [][]),
-                            prove(``∀x y l1 l2. PERM l1 l2 ==>
-                                                PERM (x::y::l1) (y::x::l2)``,
+                            prove(“∀x y l1 l2. PERM l1 l2 ==>
+                                                PERM (x::y::l1) (y::x::l2)”,
                                   SRW_TAC [][PERM_SWAP_AT_FRONT]),
                             PERM_TRANS]
 val strong_perm_ind = IndDefLib.derive_strong_induction (PERM_RULES, PERM_IND)
 
 val valid_ctxt_PERM = store_thm(
   "valid_ctxt_PERM",
-  ``!G1 G2. PERM G1 G2 ==> (valid_ctxt G1 = valid_ctxt G2)``,
+  “!G1 G2. PERM G1 G2 ==> (valid_ctxt G1 = valid_ctxt G2)”,
   HO_MATCH_MP_TAC strong_perm_ind THEN
   SIMP_TAC (srw_ss()) [pairTheory.FORALL_PROD, NOT_IN_supp_listpm] THEN
   SRW_TAC [][] THEN METIS_TAC [PERM_MEM_EQ]);
 
 val valid_ctxt_FILTER = store_thm(
   "valid_ctxt_FILTER",
-  ``valid_ctxt G ==> valid_ctxt (FILTER P G)``,
-  Induct_on `G` THEN
+  “valid_ctxt G ==> valid_ctxt (FILTER P G)”,
+  Induct_on ‘G’ THEN
   SIMP_TAC (srw_ss()) [pairTheory.FORALL_PROD, NOT_IN_supp_listpm] THEN
   SRW_TAC [][IN_supp_listpm, pairTheory.EXISTS_PROD, listTheory.MEM_FILTER]);
-val domfilter_def = Define`
+val domfilter_def = Define‘
   domfilter (G:'a ctxt) P = FILTER (λ(x,ty). x ∈ P) G
-`;
-val _ = overload_on ("INTER", ``domfilter``)
+’;
+val _ = overload_on ("INTER", “domfilter”)
 
 val domfilter_thm = store_thm(
   "domfilter_thm",
-  ``([] ∩ P = []) ∧
-    ((h :: G) ∩ P = if FST h ∈ P then h :: (G ∩ P) else G ∩ P)``,
-  Cases_on `h` THEN SRW_TAC [][domfilter_def])
+  “([] ∩ P = []) ∧
+    ((h :: G) ∩ P = if FST h ∈ P then h :: (G ∩ P) else G ∩ P)”,
+  Cases_on ‘h’ THEN SRW_TAC [][domfilter_def])
 val _ = export_rewrites ["domfilter_thm"]
 
 val valid_ctxt_domfilter = store_thm(
   "valid_ctxt_domfilter",
-  ``valid_ctxt G ==> valid_ctxt (G ∩ P)``,
+  “valid_ctxt G ==> valid_ctxt (G ∩ P)”,
   SRW_TAC [][domfilter_def, valid_ctxt_FILTER]);
 
 val IN_ctxtFV_domfilter = store_thm(
   "IN_ctxtFV_domfilter",
-  ``x ∈ ctxtFV (G ∩ P) ⇔ x ∈ ctxtFV G ∧ x ∈ P``,
-  Induct_on `G` THEN ASM_SIMP_TAC (srw_ss()) [pairTheory.FORALL_PROD] THEN
+  “x ∈ ctxtFV (G ∩ P) ⇔ x ∈ ctxtFV G ∧ x ∈ P”,
+  Induct_on ‘G’ THEN ASM_SIMP_TAC (srw_ss()) [pairTheory.FORALL_PROD] THEN
   SRW_TAC [][] THEN METIS_TAC []);
 val _ = export_rewrites ["IN_ctxtFV_domfilter"]
 
@@ -157,12 +148,12 @@ QED
 
 val subctxt_domfilter = store_thm(
   "subctxt_domfilter",
-  ``(G:'a ctxt) ∩ P ⊆ G``,
+  “(G:'a ctxt) ∩ P ⊆ G”,
   SRW_TAC [][subctxt_def, domfilter_def, listTheory.MEM_FILTER]);
 
 val domfilter_delete = store_thm(
   "domfilter_delete",
-  ``¬(v ∈ ctxtFV G) ==> (G ∩ (s DELETE v) = G ∩ s)``,
-  Induct_on `G` THEN ASM_SIMP_TAC (srw_ss()) [pairTheory.FORALL_PROD]);
+  “¬(v ∈ ctxtFV G) ==> (G ∩ (s DELETE v) = G ∩ s)”,
+  Induct_on ‘G’ THEN ASM_SIMP_TAC (srw_ss()) [pairTheory.FORALL_PROD]);
 
 val _ = export_theory()
